make unknown_match_tac take the (preliminary) decision into account

SemanticsTernary/Matching_Ternary.thy
@@ -12,7 +12,7 @@ text\<open>
 If the matching is @{const TernaryUnknown}, it can be decided by the action whether this rule matches.
 E.g. in doubt, we allow packets
 \<close>
-type_synonym 'packet unknown_match_tac="action \<Rightarrow> 'packet \<Rightarrow> bool"
+type_synonym 'packet unknown_match_tac="action \<Rightarrow> decision \<Rightarrow> 'packet \<Rightarrow> bool"
 
 type_synonym ('a, 'packet) match_tac="(('a, 'packet) exact_match_tac \<times> 'packet unknown_match_tac)"
 
@@ -41,10 +41,10 @@ begin
 end
 
 
-fun ternary_to_bool_unknown_match_tac :: "'packet unknown_match_tac \<Rightarrow> action \<Rightarrow> 'packet \<Rightarrow> ternaryvalue \<Rightarrow> bool" where
-  "ternary_to_bool_unknown_match_tac _ _ _ TernaryTrue = True" |
-  "ternary_to_bool_unknown_match_tac _ _ _ TernaryFalse = False" |
-  "ternary_to_bool_unknown_match_tac \<alpha> a p TernaryUnknown = \<alpha> a p"
+fun ternary_to_bool_unknown_match_tac :: "'packet unknown_match_tac \<Rightarrow> action \<Rightarrow> decision \<Rightarrow> 'packet \<Rightarrow> ternaryvalue \<Rightarrow> bool" where
+  "ternary_to_bool_unknown_match_tac _ _ _ _ TernaryTrue = True" |
+  "ternary_to_bool_unknown_match_tac _ _ _ _ TernaryFalse = False" |
+  "ternary_to_bool_unknown_match_tac \<alpha> a d p TernaryUnknown = \<alpha> a d p"
 
 text\<open>
 Matching a packet and a rule:
@@ -55,23 +55,23 @@ Matching a packet and a rule:
   \item If @{const TernaryUnknown}, apply the @{typ "'a unknown_match_tac"} to get a Boolean result
 \end{enumerate}
 \<close>
-definition matches :: "('a, 'packet) match_tac \<Rightarrow> 'a match_expr \<Rightarrow> action \<Rightarrow> 'packet \<Rightarrow> bool" where
-  "matches \<gamma> m a p \<equiv> ternary_to_bool_unknown_match_tac (snd \<gamma>) a p (ternary_ternary_eval (map_match_tac (fst \<gamma>) p m))"
+definition matches :: "('a, 'packet) match_tac \<Rightarrow> 'a match_expr \<Rightarrow> action \<Rightarrow> decision \<Rightarrow> 'packet \<Rightarrow> bool" where
+  "matches \<gamma> m a d p \<equiv> ternary_to_bool_unknown_match_tac (snd \<gamma>) a d p (ternary_ternary_eval (map_match_tac (fst \<gamma>) p m))"
 
 text\<open>Alternative matches definitions, some more or less convenient\<close>
 
-lemma matches_tuple: "matches (\<beta>, \<alpha>) m a p = ternary_to_bool_unknown_match_tac \<alpha> a p (ternary_ternary_eval (map_match_tac \<beta> p m))"
+lemma matches_tuple: "matches (\<beta>, \<alpha>) m a d p = ternary_to_bool_unknown_match_tac \<alpha> a d p (ternary_ternary_eval (map_match_tac \<beta> p m))"
 unfolding matches_def by simp
 
-lemma matches_case: "matches \<gamma> m a p \<longleftrightarrow> (case ternary_eval (map_match_tac (fst \<gamma>) p m) of None \<Rightarrow> (snd \<gamma>) a p | Some b \<Rightarrow> b)"
+lemma matches_case: "matches \<gamma> m a d p \<longleftrightarrow> (case ternary_eval (map_match_tac (fst \<gamma>) p m) of None \<Rightarrow> (snd \<gamma>) a d p | Some b \<Rightarrow> b)"
 unfolding matches_def ternary_eval_def
 by (cases "(ternary_ternary_eval (map_match_tac (fst \<gamma>) p m))") auto
 
-lemma matches_case_tuple: "matches (\<beta>, \<alpha>) m a p \<longleftrightarrow> (case ternary_eval (map_match_tac \<beta> p m) of None \<Rightarrow> \<alpha> a p | Some b \<Rightarrow> b)"
+lemma matches_case_tuple: "matches (\<beta>, \<alpha>) m a d p \<longleftrightarrow> (case ternary_eval (map_match_tac \<beta> p m) of None \<Rightarrow> \<alpha> a d p | Some b \<Rightarrow> b)"
 by (auto simp: matches_case split: option.splits)
 
-lemma matches_case_ternaryvalue_tuple: "matches (\<beta>, \<alpha>) m a p \<longleftrightarrow> (case ternary_ternary_eval (map_match_tac \<beta> p m) of 
-        TernaryUnknown \<Rightarrow> \<alpha> a p | 
+lemma matches_case_ternaryvalue_tuple: "matches (\<beta>, \<alpha>) m a d p \<longleftrightarrow> (case ternary_ternary_eval (map_match_tac \<beta> p m) of 
+        TernaryUnknown \<Rightarrow> \<alpha> a d p | 
         TernaryTrue \<Rightarrow> True |
         TernaryFalse \<Rightarrow> False)"
   by(simp split: option.split ternaryvalue.split add: matches_case ternary_to_bool_None ternary_eval_def)
@@ -79,8 +79,8 @@ lemma matches_case_ternaryvalue_tuple: "matches (\<beta>, \<alpha>) m a p \<long
 
 
 lemma matches_casesE:
-  "matches (\<beta>, \<alpha>) m a p \<Longrightarrow> 
-    (ternary_ternary_eval (map_match_tac \<beta> p m) = TernaryUnknown \<Longrightarrow> \<alpha> a p \<Longrightarrow> P) \<Longrightarrow> 
+  "matches (\<beta>, \<alpha>) m a d p \<Longrightarrow> 
+    (ternary_ternary_eval (map_match_tac \<beta> p m) = TernaryUnknown \<Longrightarrow> \<alpha> a d p \<Longrightarrow> P) \<Longrightarrow> 
     (ternary_ternary_eval (map_match_tac \<beta> p m) = TernaryTrue \<Longrightarrow> P)
   \<Longrightarrow> P"
 proof(induction m)
@@ -90,44 +90,44 @@ qed(auto split: option.split_asm simp: matches_case_tuple ternary_eval_def terna
 text\<open>
 Example: @{text "\<not> Unknown"} is as good as @{text Unknown}
 \<close>
-lemma "\<lbrakk> ternary_ternary_eval (map_match_tac \<beta> p expr) = TernaryUnknown \<rbrakk> \<Longrightarrow> matches (\<beta>, \<alpha>) expr a p \<longleftrightarrow> matches (\<beta>, \<alpha>) (MatchNot expr) a p"
+lemma "\<lbrakk> ternary_ternary_eval (map_match_tac \<beta> p expr) = TernaryUnknown \<rbrakk> \<Longrightarrow> matches (\<beta>, \<alpha>) expr a d p \<longleftrightarrow> matches (\<beta>, \<alpha>) (MatchNot expr) a d p"
 by(simp add: matches_case_ternaryvalue_tuple)
 
 
 lemma bunch_of_lemmata_about_matches:
-  "matches \<gamma> (MatchAnd m1 m2) a p \<longleftrightarrow> matches \<gamma> m1 a p \<and> matches \<gamma> m2 a p" (*split AND*)
-  "matches \<gamma> MatchAny a p" (*MatchAny is True*)
-  "matches \<gamma> (MatchNot MatchAny) a p \<longleftrightarrow> False" (*Not True*)
-  "matches \<gamma> (MatchNot (MatchNot m)) a p \<longleftrightarrow> matches \<gamma> m a p" (*idempotence*)
+  "matches \<gamma> (MatchAnd m1 m2) a d p \<longleftrightarrow> matches \<gamma> m1 a d p \<and> matches \<gamma> m2 a d p" (*split AND*)
+  "matches \<gamma> MatchAny a d p" (*MatchAny is True*)
+  "matches \<gamma> (MatchNot MatchAny) a d p \<longleftrightarrow> False" (*Not True*)
+  "matches \<gamma> (MatchNot (MatchNot m)) a d p \<longleftrightarrow> matches \<gamma> m a d p" (*idempotence*)
 proof(case_tac [!] \<gamma>)
 qed (simp_all split: ternaryvalue.split add: matches_case_ternaryvalue_tuple)
 
 lemma match_raw_bool:
-  "matches (\<beta>, \<alpha>) (Match expr) a p = (case ternary_to_bool (\<beta> expr p) of Some r \<Rightarrow> r | None \<Rightarrow> (\<alpha> a p))" (*Match raw*)
+  "matches (\<beta>, \<alpha>) (Match expr) a d p = (case ternary_to_bool (\<beta> expr p) of Some r \<Rightarrow> r | None \<Rightarrow> (\<alpha> a d p))" (*Match raw*)
 by(simp_all split: ternaryvalue.split add: matches_case_ternaryvalue_tuple)
 lemma match_raw_ternary:
-  "matches (\<beta>, \<alpha>) (Match expr) a p = (case (\<beta> expr p) of TernaryTrue \<Rightarrow> True | TernaryFalse \<Rightarrow> False | TernaryUnknown \<Rightarrow> (\<alpha> a p))" (*Match raw explicit*)
+  "matches (\<beta>, \<alpha>) (Match expr) a d p = (case (\<beta> expr p) of TernaryTrue \<Rightarrow> True | TernaryFalse \<Rightarrow> False | TernaryUnknown \<Rightarrow> (\<alpha> a d p))" (*Match raw explicit*)
 by(simp_all split: ternaryvalue.split add: matches_case_ternaryvalue_tuple)
 
 (*kind of the DeMorgan Rule for matches*)
-lemma matches_DeMorgan: "matches \<gamma> (MatchNot (MatchAnd m1 m2)) a p \<longleftrightarrow> (matches \<gamma> (MatchNot m1) a p) \<or> (matches \<gamma> (MatchNot m2) a p)"
+lemma matches_DeMorgan: "matches \<gamma> (MatchNot (MatchAnd m1 m2)) a d p \<longleftrightarrow> (matches \<gamma> (MatchNot m1) a d p) \<or> (matches \<gamma> (MatchNot m2) a d p)"
 by (cases \<gamma>) (simp split: ternaryvalue.split add: matches_case_ternaryvalue_tuple eval_ternary_DeMorgan)
 
 
 subsection\<open>Ternary Matcher Algebra\<close>
 
-lemma matches_and_comm: "matches \<gamma> (MatchAnd m m') a p \<longleftrightarrow> matches \<gamma> (MatchAnd m' m) a p"
+lemma matches_and_comm: "matches \<gamma> (MatchAnd m m') a d p \<longleftrightarrow> matches \<gamma> (MatchAnd m' m) a d p"
 apply(cases \<gamma>, rename_tac \<beta> \<alpha>, clarify)
 by(simp add: matches_case_ternaryvalue_tuple eval_ternary_And_comm)
 
-lemma matches_not_idem: "matches \<gamma> (MatchNot (MatchNot m)) a p \<longleftrightarrow> matches \<gamma> m a p"
+lemma matches_not_idem: "matches \<gamma> (MatchNot (MatchNot m)) a d p \<longleftrightarrow> matches \<gamma> m a d p"
 by (fact bunch_of_lemmata_about_matches)
 
 
-lemma MatchOr: "matches \<gamma> (MatchOr m1 m2) a p \<longleftrightarrow> matches \<gamma> m1 a p \<or> matches \<gamma> m2 a p"
+lemma MatchOr: "matches \<gamma> (MatchOr m1 m2) a d p \<longleftrightarrow> matches \<gamma> m1 a d p \<or> matches \<gamma> m2 a d p"
   by(simp add: MatchOr_def matches_DeMorgan matches_not_idem)
 
-lemma MatchOr_MatchNot: "matches \<gamma> (MatchNot (MatchOr m1 m2)) a p \<longleftrightarrow> matches \<gamma> (MatchNot m1) a p \<and> matches \<gamma> (MatchNot m2) a p"
+lemma MatchOr_MatchNot: "matches \<gamma> (MatchNot (MatchOr m1 m2)) a d p \<longleftrightarrow> matches \<gamma> (MatchNot m1) a d p \<and> matches \<gamma> (MatchNot m2) a d p"
   by(simp add: MatchOr_def matches_DeMorgan bunch_of_lemmata_about_matches)
 
 lemma "(TernaryNot (map_match_tac \<beta> p (m))) = (map_match_tac \<beta> p (MatchNot m))"
@@ -135,25 +135,25 @@ by (metis map_match_tac.simps(2))
 
 context
 begin
-  private lemma matches_simp1: "matches \<gamma> m a p \<Longrightarrow> matches \<gamma> (MatchAnd m m') a p \<longleftrightarrow> matches \<gamma> m' a p"
+  private lemma matches_simp1: "matches \<gamma> m a d p \<Longrightarrow> matches \<gamma> (MatchAnd m m') a d p \<longleftrightarrow> matches \<gamma> m' a d p"
     apply(cases \<gamma>, rename_tac \<beta> \<alpha>, clarify)
     apply(simp split: ternaryvalue.split_asm ternaryvalue.split add: matches_case_ternaryvalue_tuple)
     done
   
-  private lemma matches_simp11: "matches \<gamma> m a p \<Longrightarrow> matches \<gamma> (MatchAnd m' m) a p \<longleftrightarrow> matches \<gamma> m' a p"
+  private lemma matches_simp11: "matches \<gamma> m a d p \<Longrightarrow> matches \<gamma> (MatchAnd m' m) a d p \<longleftrightarrow> matches \<gamma> m' a d p"
     by(simp_all add: matches_and_comm matches_simp1)
   
-  private lemma matches_simp2: "matches \<gamma> (MatchAnd m m') a p \<Longrightarrow> \<not> matches \<gamma> m a p \<Longrightarrow> False"
+  private lemma matches_simp2: "matches \<gamma> (MatchAnd m m') a d p \<Longrightarrow> \<not> matches \<gamma> m a d p \<Longrightarrow> False"
     by (simp add: bunch_of_lemmata_about_matches)
-  private lemma matches_simp22: "matches \<gamma> (MatchAnd m m') a p \<Longrightarrow> \<not> matches \<gamma> m' a p \<Longrightarrow> False"
+  private lemma matches_simp22: "matches \<gamma> (MatchAnd m m') a d p \<Longrightarrow> \<not> matches \<gamma> m' a d p \<Longrightarrow> False"
     by (simp add: bunch_of_lemmata_about_matches)
   
   (*m simplifies to MatchUnknown*)
- private  lemma matches_simp3: "matches \<gamma> (MatchNot m) a p \<Longrightarrow> matches \<gamma> m a p \<Longrightarrow> (snd \<gamma>) a p"
+ private  lemma matches_simp3: "matches \<gamma> (MatchNot m) a d p \<Longrightarrow> matches \<gamma> m a d p \<Longrightarrow> (snd \<gamma>) a d p"
     apply(cases \<gamma>, rename_tac \<beta> \<alpha>, clarify)
     apply(simp split: ternaryvalue.split_asm ternaryvalue.split add: matches_case_ternaryvalue_tuple)
     done
-  private lemma "matches \<gamma> (MatchNot m) a p \<Longrightarrow> matches \<gamma> m a p \<Longrightarrow> (ternary_eval (map_match_tac (fst \<gamma>) p m)) = None"
+  private lemma "matches \<gamma> (MatchNot m) a d p \<Longrightarrow> matches \<gamma> m a d p \<Longrightarrow> (ternary_eval (map_match_tac (fst \<gamma>) p m)) = None"
     apply(cases \<gamma>, rename_tac \<beta> \<alpha>, clarify)
     apply(simp split: ternaryvalue.split_asm ternaryvalue.split add: matches_case_ternaryvalue_tuple ternary_eval_def)
     done
@@ -163,52 +163,52 @@ begin
 end
 
 
-lemma matches_iff_apply_f_generic: "ternary_ternary_eval (map_match_tac \<beta> p (f (\<beta>,\<alpha>) a m)) = ternary_ternary_eval (map_match_tac \<beta> p m) \<Longrightarrow> matches (\<beta>,\<alpha>) (f (\<beta>,\<alpha>) a m) a p \<longleftrightarrow> matches (\<beta>,\<alpha>) m a p"
+lemma matches_iff_apply_f_generic: "ternary_ternary_eval (map_match_tac \<beta> p (f (\<beta>,\<alpha>) a m)) = ternary_ternary_eval (map_match_tac \<beta> p m) \<Longrightarrow> matches (\<beta>,\<alpha>) (f (\<beta>,\<alpha>) a m) a d p \<longleftrightarrow> matches (\<beta>,\<alpha>) m a d p"
   by(simp split: ternaryvalue.split_asm ternaryvalue.split add: matches_case_ternaryvalue_tuple)
 
-lemma matches_iff_apply_f: "ternary_ternary_eval (map_match_tac \<beta> p (f m)) = ternary_ternary_eval (map_match_tac \<beta> p m) \<Longrightarrow> matches (\<beta>,\<alpha>) (f m) a p \<longleftrightarrow> matches (\<beta>,\<alpha>) m a p"
+lemma matches_iff_apply_f: "ternary_ternary_eval (map_match_tac \<beta> p (f m)) = ternary_ternary_eval (map_match_tac \<beta> p m) \<Longrightarrow> matches (\<beta>,\<alpha>) (f m) a d p \<longleftrightarrow> matches (\<beta>,\<alpha>) m a d p"
   by(fact matches_iff_apply_f_generic)
 
 subsection\<open>Removing Unknown Primitives\<close>
 
-definition unknown_match_all :: "'a unknown_match_tac \<Rightarrow> action \<Rightarrow> bool" where
-   "unknown_match_all \<alpha> a = (\<forall>p. \<alpha> a p)"
-definition unknown_not_match_any :: "'a unknown_match_tac \<Rightarrow> action \<Rightarrow> bool" where
-   "unknown_not_match_any \<alpha> a = (\<forall>p. \<not> \<alpha> a p)"
+definition unknown_match_all :: "'a unknown_match_tac \<Rightarrow> action \<Rightarrow> decision \<Rightarrow> bool" where
+   "unknown_match_all \<alpha> a d = (\<forall>p. \<alpha> a d p)"
+definition unknown_not_match_any :: "'a unknown_match_tac \<Rightarrow> action \<Rightarrow> decision \<Rightarrow> bool" where
+   "unknown_not_match_any \<alpha> a d = (\<forall>p. \<not> \<alpha> a d p)"
 
 (*see upper_closure_matchexpr*)
-fun remove_unknowns_generic :: "('a, 'packet) match_tac \<Rightarrow> action \<Rightarrow> 'a match_expr \<Rightarrow> 'a match_expr" where
-  "remove_unknowns_generic _ _ MatchAny = MatchAny" |
-  "remove_unknowns_generic _ _ (MatchNot MatchAny) = MatchNot MatchAny" |
-  "remove_unknowns_generic (\<beta>, \<alpha>) a (Match A) = (if
+fun remove_unknowns_generic :: "('a, 'packet) match_tac \<Rightarrow> action \<Rightarrow> decision \<Rightarrow> 'a match_expr \<Rightarrow> 'a match_expr" where
+  "remove_unknowns_generic _ _ _ MatchAny = MatchAny" |
+  "remove_unknowns_generic _ _ _ (MatchNot MatchAny) = MatchNot MatchAny" |
+  "remove_unknowns_generic (\<beta>, \<alpha>) a d (Match A) = (if
       (\<forall>p. ternary_ternary_eval (map_match_tac \<beta> p (Match A)) = TernaryUnknown)
     then
-      if unknown_match_all \<alpha> a then MatchAny else if unknown_not_match_any \<alpha> a then MatchNot MatchAny else Match A
+      if unknown_match_all \<alpha> a d then MatchAny else if unknown_not_match_any \<alpha> a d then MatchNot MatchAny else Match A
     else (Match A))" |
-  "remove_unknowns_generic (\<beta>, \<alpha>) a (MatchNot (Match A)) = (if
+  "remove_unknowns_generic (\<beta>, \<alpha>) a d (MatchNot (Match A)) = (if
       (\<forall>p. ternary_ternary_eval (map_match_tac \<beta> p (Match A)) = TernaryUnknown)
     then
-      if unknown_match_all \<alpha> a then MatchAny else if unknown_not_match_any \<alpha> a then MatchNot MatchAny else MatchNot (Match A)
+      if unknown_match_all \<alpha> a d then MatchAny else if unknown_not_match_any \<alpha> a d then MatchNot MatchAny else MatchNot (Match A)
     else MatchNot (Match A))" |
-  "remove_unknowns_generic (\<beta>, \<alpha>) a (MatchNot (MatchNot m)) = remove_unknowns_generic (\<beta>, \<alpha>) a m" |
-  "remove_unknowns_generic (\<beta>, \<alpha>) a (MatchAnd m1 m2) = MatchAnd
-      (remove_unknowns_generic (\<beta>, \<alpha>) a m1)
-      (remove_unknowns_generic (\<beta>, \<alpha>) a m2)" |
+  "remove_unknowns_generic (\<beta>, \<alpha>) a d (MatchNot (MatchNot m)) = remove_unknowns_generic (\<beta>, \<alpha>) a d m" |
+  "remove_unknowns_generic (\<beta>, \<alpha>) a d (MatchAnd m1 m2) = MatchAnd
+      (remove_unknowns_generic (\<beta>, \<alpha>) a d m1)
+      (remove_unknowns_generic (\<beta>, \<alpha>) a d m2)" |
 
   --\<open>@{text "\<not> (a \<and> b) = \<not> b \<or> \<not> a"}   and   @{text "\<not> Unknown = Unknown"}\<close>
-  "remove_unknowns_generic (\<beta>, \<alpha>) a (MatchNot (MatchAnd m1 m2)) = 
-    (if (remove_unknowns_generic (\<beta>, \<alpha>) a (MatchNot m1)) = MatchAny \<or>
-        (remove_unknowns_generic (\<beta>, \<alpha>) a (MatchNot m2)) = MatchAny
+  "remove_unknowns_generic (\<beta>, \<alpha>) a d (MatchNot (MatchAnd m1 m2)) = 
+    (if (remove_unknowns_generic (\<beta>, \<alpha>) a d (MatchNot m1)) = MatchAny \<or>
+        (remove_unknowns_generic (\<beta>, \<alpha>) a d (MatchNot m2)) = MatchAny
         then MatchAny else 
-        (if (remove_unknowns_generic (\<beta>, \<alpha>) a (MatchNot m1)) = MatchNot MatchAny then 
-          remove_unknowns_generic (\<beta>, \<alpha>) a (MatchNot m2) else
-         if (remove_unknowns_generic (\<beta>, \<alpha>) a (MatchNot m2)) = MatchNot MatchAny then 
-          remove_unknowns_generic (\<beta>, \<alpha>) a (MatchNot m1) else
-         MatchNot (MatchAnd (MatchNot (remove_unknowns_generic (\<beta>, \<alpha>) a (MatchNot m1))) (MatchNot (remove_unknowns_generic (\<beta>, \<alpha>) a (MatchNot m2)))))
+        (if (remove_unknowns_generic (\<beta>, \<alpha>) a d (MatchNot m1)) = MatchNot MatchAny then 
+          remove_unknowns_generic (\<beta>, \<alpha>) a d (MatchNot m2) else
+         if (remove_unknowns_generic (\<beta>, \<alpha>) a d (MatchNot m2)) = MatchNot MatchAny then 
+          remove_unknowns_generic (\<beta>, \<alpha>) a d (MatchNot m1) else
+         MatchNot (MatchAnd (MatchNot (remove_unknowns_generic (\<beta>, \<alpha>) a d (MatchNot m1))) (MatchNot (remove_unknowns_generic (\<beta>, \<alpha>) a d (MatchNot m2)))))
        )"
 
-lemma[code_unfold]: "remove_unknowns_generic \<gamma> a (MatchNot (MatchAnd m1 m2)) = 
-    (let m1' = remove_unknowns_generic \<gamma>  a (MatchNot m1); m2' = remove_unknowns_generic \<gamma>  a (MatchNot m2) in
+lemma[code_unfold]: "remove_unknowns_generic \<gamma> a d (MatchNot (MatchAnd m1 m2)) = 
+    (let m1' = remove_unknowns_generic \<gamma>  a d (MatchNot m1); m2' = remove_unknowns_generic \<gamma>  a d (MatchNot m2) in
     (if m1' = MatchAny \<or> m2' = MatchAny
      then MatchAny
      else 
@@ -220,15 +220,15 @@ lemma[code_unfold]: "remove_unknowns_generic \<gamma> a (MatchNot (MatchAnd m1 m
 by(cases \<gamma>)(simp)
 
 
-lemma remove_unknowns_generic_simp_3_4_unfolded: "remove_unknowns_generic (\<beta>, \<alpha>) a (Match A) = (if
+lemma remove_unknowns_generic_simp_3_4_unfolded: "remove_unknowns_generic (\<beta>, \<alpha>) a d (Match A) = (if
       (\<forall>p. ternary_ternary_eval (map_match_tac \<beta> p (Match A)) = TernaryUnknown)
     then
-      if (\<forall>p. \<alpha> a p) then MatchAny else if (\<forall>p. \<not> \<alpha> a p) then MatchNot MatchAny else Match A
+      if (\<forall>p. \<alpha> a d p) then MatchAny else if (\<forall>p. \<not> \<alpha> a d p) then MatchNot MatchAny else Match A
     else (Match A))" 
- "remove_unknowns_generic (\<beta>, \<alpha>) a (MatchNot (Match A)) = (if
+ "remove_unknowns_generic (\<beta>, \<alpha>) a d (MatchNot (Match A)) = (if
       (\<forall>p. ternary_ternary_eval (map_match_tac \<beta> p (Match A)) = TernaryUnknown)
     then
-      if (\<forall>p. \<alpha> a p) then MatchAny else if (\<forall>p. \<not> \<alpha> a p) then MatchNot MatchAny else MatchNot (Match A)
+      if (\<forall>p. \<alpha> a d p) then MatchAny else if (\<forall>p. \<not> \<alpha> a d p) then MatchNot MatchAny else MatchNot (Match A)
     else MatchNot (Match A))"
   by(auto simp add: unknown_match_all_def unknown_not_match_any_def)
 
@@ -239,16 +239,16 @@ lemmas remove_unknowns_generic_simps2 = remove_unknowns_generic.simps(1) remove_
             remove_unknowns_generic.simps(5) remove_unknowns_generic.simps(6) remove_unknowns_generic.simps(7)
 
 
-lemma "matches (\<beta>, \<alpha>) (remove_unknowns_generic (\<beta>, \<alpha>) a (MatchNot (Match A))) a p = matches (\<beta>, \<alpha>) (MatchNot (Match A)) a p"
+lemma "matches (\<beta>, \<alpha>) (remove_unknowns_generic (\<beta>, \<alpha>) a d (MatchNot (Match A))) a d p = matches (\<beta>, \<alpha>) (MatchNot (Match A)) a d p"
 by(simp add: remove_unknowns_generic_simps2 matches_case_ternaryvalue_tuple)
 
 
 
-lemma remove_unknowns_generic: "matches \<gamma> (remove_unknowns_generic \<gamma> a m) a = matches \<gamma> m a"
+lemma remove_unknowns_generic: "matches \<gamma> (remove_unknowns_generic \<gamma> a d m) a d = matches \<gamma> m a d"
 proof -
-  have "matches \<gamma> (remove_unknowns_generic \<gamma> a m) a p = matches \<gamma> m a p"
+  have "matches \<gamma> (remove_unknowns_generic \<gamma> a d m) a d p = matches \<gamma> m a d p"
   for p
-  proof(induction \<gamma> a m rule: remove_unknowns_generic.induct)
+  proof(induction \<gamma> a d m rule: remove_unknowns_generic.induct)
   case 3 thus ?case
       by(simp add: bunch_of_lemmata_about_matches match_raw_ternary remove_unknowns_generic_simps2)
   next
@@ -274,9 +274,9 @@ fun has_unknowns :: " ('a, 'p) exact_match_tac \<Rightarrow> 'a match_expr \<Rig
   "has_unknowns \<beta> (MatchAnd m1 m2) = (has_unknowns \<beta> m1 \<or> has_unknowns \<beta> m2)"
 
 definition packet_independent_\<alpha> :: "'p unknown_match_tac \<Rightarrow> bool" where
-  "packet_independent_\<alpha> \<alpha> = (\<forall>a p1 p2. a=Pass \<or> a=Block \<longrightarrow> \<alpha> a p1 \<longleftrightarrow> \<alpha> a p2)"
+  "packet_independent_\<alpha> \<alpha> = (\<forall>a d p1 p2. a=Pass \<or> a=Block \<longrightarrow> \<alpha> a d p1 \<longleftrightarrow> \<alpha> a d p2)"
 
-lemma packet_independent_unknown_match: "a=Pass \<or> a=Block \<Longrightarrow> packet_independent_\<alpha> \<alpha> \<Longrightarrow> \<not> unknown_not_match_any \<alpha> a \<longleftrightarrow> unknown_match_all \<alpha> a"
+lemma packet_independent_unknown_match: "a=Pass \<or> a=Block \<Longrightarrow> packet_independent_\<alpha> \<alpha> \<Longrightarrow> \<not> unknown_not_match_any \<alpha> a d \<longleftrightarrow> unknown_match_all \<alpha> a d"
   by(auto simp add: packet_independent_\<alpha>_def unknown_match_all_def unknown_not_match_any_def)
 
 text\<open>If for some type the exact matcher returns unknown, then it returns unknown for all these types\<close>
@@ -286,8 +286,8 @@ definition packet_independent_\<beta>_unknown :: "('a, 'packet) exact_match_tac 
 
 lemma remove_unknowns_generic_specification: "a=Pass \<or> a=Block \<Longrightarrow> packet_independent_\<alpha> \<alpha> \<Longrightarrow>
   packet_independent_\<beta>_unknown \<beta> \<Longrightarrow>
-   \<not> has_unknowns \<beta> (remove_unknowns_generic (\<beta>, \<alpha>) a m)"
-  proof(induction "(\<beta>, \<alpha>)" a m rule: remove_unknowns_generic.induct)
+   \<not> has_unknowns \<beta> (remove_unknowns_generic (\<beta>, \<alpha>) a d m)"
+  proof(induction "(\<beta>, \<alpha>)" a d m rule: remove_unknowns_generic.induct)
   case 3 thus ?case by(simp add: packet_independent_unknown_match packet_independent_\<beta>_unknown_def remove_unknowns_generic.simps)
   next
   case 4 thus ?case by(simp add: packet_independent_unknown_match packet_independent_\<beta>_unknown_def remove_unknowns_generic.simps)
@@ -312,11 +312,11 @@ begin
   qed
 
 
-  private lemma no_primitives_matchNot: assumes "\<not> has_primitive m" shows "matches \<gamma> (MatchNot m) a p \<longleftrightarrow> \<not> matches \<gamma> m a p"
+  private lemma no_primitives_matchNot: assumes "\<not> has_primitive m" shows "matches \<gamma> (MatchNot m) a d p \<longleftrightarrow> \<not> matches \<gamma> m a d p"
   proof -
     obtain \<beta> \<alpha> where "(\<beta>, \<alpha>) = \<gamma>" by (cases \<gamma>, simp)
     thm no_primitives_no_unknown
-    from assms have "matches (\<beta>, \<alpha>) (MatchNot m) a p \<longleftrightarrow> \<not> matches (\<beta>, \<alpha>) m a p"
+    from assms have "matches (\<beta>, \<alpha>) (MatchNot m) a d p \<longleftrightarrow> \<not> matches (\<beta>, \<alpha>) m a d p"
       apply(induction m)
          apply(simp_all add: matches_case_ternaryvalue_tuple split: ternaryvalue.split )
       apply(rename_tac m1 m2)
@@ -325,14 +325,14 @@ begin
   qed
   
 
-  lemma matcheq_matchAny: "\<not> has_primitive m \<Longrightarrow> matcheq_matchAny m \<longleftrightarrow> matches \<gamma> m a p"
+  lemma matcheq_matchAny: "\<not> has_primitive m \<Longrightarrow> matcheq_matchAny m \<longleftrightarrow> matches \<gamma> m a d p"
   proof(induction m)
   case Match hence False by auto
     thus ?case ..
   next
   case (MatchNot m)
     from MatchNot.prems have "\<not> has_primitive m" by simp
-    with no_primitives_matchNot have "matches \<gamma> (MatchNot m) a p = (\<not> matches \<gamma> m a p)" by metis
+    with no_primitives_matchNot have "matches \<gamma> (MatchNot m) a d p = (\<not> matches \<gamma> m a d p)" by metis
     with MatchNot show ?case by(simp)
   next
   case (MatchAnd m1 m2)
@@ -341,10 +341,10 @@ begin
   case MatchAny show ?case by(simp add: Matching_Ternary.bunch_of_lemmata_about_matches)
   qed
 
-  lemma matcheq_matchNone: "\<not> has_primitive m \<Longrightarrow> matcheq_matchNone m \<longleftrightarrow> \<not> matches \<gamma> m a p"
+  lemma matcheq_matchNone: "\<not> has_primitive m \<Longrightarrow> matcheq_matchNone m \<longleftrightarrow> \<not> matches \<gamma> m a d p"
     by(auto dest: matcheq_matchAny matachAny_matchNone)
 
-  lemma matcheq_matchNone_not_matches: "matcheq_matchNone m \<Longrightarrow> \<not> matches \<gamma> m a p"
+  lemma matcheq_matchNone_not_matches: "matcheq_matchNone m \<Longrightarrow> \<not> matches \<gamma> m a d p"
     proof(induction m rule: matcheq_matchNone.induct)
     qed(auto simp add: bunch_of_lemmata_about_matches matches_DeMorgan)
     
@@ -356,7 +356,7 @@ text\<open>Lemmas about @{const MatchNot} in ternary logic.\<close>
 
 lemma matches_MatchNot_no_unknowns:
    assumes "\<not> has_unknowns \<beta> m"
-   shows "matches (\<beta>,\<alpha>) (MatchNot m) a p \<longleftrightarrow> \<not> matches (\<beta>,\<alpha>) m a p"
+   shows "matches (\<beta>,\<alpha>) (MatchNot m) a d p \<longleftrightarrow> \<not> matches (\<beta>,\<alpha>) m a d p"
 proof -
   { fix m have "\<not> has_unknowns \<beta> m \<Longrightarrow>
        ternary_to_bool (ternary_ternary_eval (map_match_tac \<beta> p m)) \<noteq> None"
@@ -373,7 +373,7 @@ proof -
 qed
 
 lemma MatchNot_ternary_ternary_eval: "(ternary_ternary_eval (map_match_tac \<beta> p m')) = (ternary_ternary_eval (map_match_tac \<beta> p m)) \<Longrightarrow>
-    matches (\<beta>,\<alpha>) (MatchNot m') a p = matches (\<beta>,\<alpha>) (MatchNot m) a p"
+    matches (\<beta>,\<alpha>) (MatchNot m') a d p = matches (\<beta>,\<alpha>) (MatchNot m) a d p"
 by(simp add: matches_tuple)
 
 
@@ -383,15 +383,15 @@ text\<open>For our @{typ "'p unknown_match_tac"}s @{text in_doubt_allow} and @{t
       we get the @{const MatchNot} case for free (if we can set arbitrary @{term "p::'p"}).
       This does not hold for arbitrary @{typ "'p unknown_match_tac"}s.\<close>
 lemma matches_induction_case_MatchNot:
-      assumes "\<alpha> Block \<noteq> \<alpha> Pass" and "packet_independent_\<alpha> \<alpha>"
-      and     "\<forall> a. matches (\<beta>,\<alpha>) m' a p = matches (\<beta>,\<alpha>) m a p"
-      shows   "matches (\<beta>,\<alpha>) (MatchNot m') a p = matches (\<beta>,\<alpha>) (MatchNot m) a p"
+      assumes "\<alpha> Block d \<noteq> \<alpha> Pass d" and "packet_independent_\<alpha> \<alpha>"
+      and     "\<forall> a. matches (\<beta>,\<alpha>) m' a d p = matches (\<beta>,\<alpha>) m a d p"
+      shows   "matches (\<beta>,\<alpha>) (MatchNot m') a d p = matches (\<beta>,\<alpha>) (MatchNot m) a d p"
 proof -
-  from assms(1) assms(2) have xxxx_xxX: "\<And>b. \<forall>a. \<alpha> a p = (\<not> b) \<Longrightarrow> False"
+  from assms(1) assms(2) have xxxx_xxX: "\<And>b. \<forall>a. \<alpha> a d p = (\<not> b) \<Longrightarrow> False"
     apply(simp add: packet_independent_\<alpha>_def)
-    apply(case_tac "\<alpha> Pass p")
+    apply(case_tac "\<alpha> Pass d p")
      apply(simp_all)
-     apply(case_tac [!] "\<alpha> Block p")
+     apply(case_tac [!] "\<alpha> Block d p")
        apply(simp_all add: fun_eq_iff)
      apply blast+
     done
